TargetSFI/MachineGen.v
@@ -1,6 +1,9 @@
+Set Implicit Arguments.
+
 Require Import ZArith.
 Require Import Coq.Lists.List.
 Require Import Coq.Strings.String.
+Require Import Notations.
 
 Require Import Common.Definitions.
 Require Import Common.Util.
@@ -64,8 +67,6 @@ Instance show_event : Show event :=
 
 Instance show_trace : Show trace := showList.
 
-Print MachineState.t.
-
 Instance show_state : Show MachineState.t :=
   {|
     show := fun (st : MachineState.t) =>
@@ -75,11 +76,12 @@ Instance show_state : Show MachineState.t :=
                      (* TODO print memory *)                     
   |}.
 
-(* TODO Arbitrary *)
-(* Generates a list of COMP_MAX+1 distinct elements *)
+
 (* TODO Use UPenn MetaLibrary *)
-Open Scope nat_scope.
-Open Scope list_scope.
+
+(*******************************
+ * Env.CN Generator
+ *******************************)
 
 Theorem decComponentId: forall x y : Component.id, {x = y} + {x <> y}.
 Proof. decide equality. Defined.
@@ -88,22 +90,241 @@ Definition cut_list (l : list Component.id) : list Component.id :=
   let fix gen_seq len :=
       match len with
       | O => [ (Pos.of_nat 1) ]
-      | S len' => (gen_seq len') ++ [ Pos.of_nat (len+1) ]
+      | S len' => List.app (gen_seq len') [ Pos.of_nat (len+1) ]
       end
   in
-  let len:nat := (N.to_nat COMP_MAX) + 1 in
+  let len:nat := (N.to_nat SFI.COMP_MAX) in
   let l' : (list Component.id) := (List.nodup decComponentId l) in 
-  if ( len <=? (List.length l') )
+  if (  Nat.leb len (List.length l') )
   then (List.firstn len l') 
   else (gen_seq len).
 
-
+Open Scope nat_scope.
 Instance genCN : Gen Env.CN :=
   {
     arbitrary :=
-      let len:nat := (N.to_nat COMP_MAX) + 1 in
-      liftGen cut_list (liftGen (map Pos.of_nat) (vectorOf (2*len) (choose (0,3*len))))
+      let len := N.to_nat SFI.COMP_MAX in
+      let double := len * 2 in
+      liftGen cut_list (liftGen (map Pos.of_nat) (vectorOf double arbitrary ))
   }.
 Close Scope nat_scope.
 
-(* Sample arbitrary. *)
+
+(*******************************
+ * Addresses Generator
+ *******************************)
+Definition genSFIComponentId : G SFIComponent.id :=
+  liftGen N.of_nat (choose (O,N.to_nat SFI.COMP_MAX)).
+
+Open Scope N_scope.
+Definition odd_even_frecv_gen (even_freq : nat) (odd_freq : nat) : G N :=
+  freq [
+      (even_freq, liftGen (fun x => 2*(N.of_nat x)) arbitrary);
+        (odd_freq, liftGen (fun x => 2*(N.of_nat x)+1) arbitrary)
+    ].
+Close Scope N_scope.
+
+Definition genBlockIds (frecv_code : nat) (frecv_data : nat) : G (list N) :=
+  let how_many : nat := plus frecv_code frecv_data in
+  vectorOf how_many (odd_even_frecv_gen frecv_code frecv_data).
+
+Definition genOffset : G N :=
+  liftGen N.of_nat (choose (O,N.to_nat SFI.get_max_offset)).
+
+Definition genBlockOffsetPairs (frecv_code : nat) (frecv_data : nat) : G (list (N*N)) :=
+  let how_many : nat := plus frecv_code frecv_data in
+  liftGen (fun '(l1,l2) => List.combine l1 l2)
+          (liftGen2 pair
+                    (genBlockIds frecv_code frecv_data)
+                    (vectorOf how_many genOffset)).
+
+Definition genAbstractAddresses (frecv_code : nat) (frecv_data : nat) :
+  G (list (SFIComponent.id*(N*N))) :=
+  let how_many := plus frecv_code frecv_data in
+  (* generator of pairs of lists cid * block id * offset *)
+  liftGen (fun '(l1,l2) => List.combine l1 l2)
+          (liftGen2 pair
+                    (vectorOf how_many genSFIComponentId)
+                    (* generator of pair of lists block id * offset *)
+                    (genBlockOffsetPairs frecv_code frecv_data)).
+
+Definition genAddresses (frecv_code : nat) (frecv_data : nat) :
+  G (list RiscMachine.address) :=
+  liftGen
+    (List.map (fun '(cid,(bid,off)) => SFI.address_of cid bid off))
+    (genAbstractAddresses frecv_code frecv_data).
+
+(* frecv_code = number of addresses in code slots
+   frecv_data = number of addresses in data slots
+   cid = the component id of all addresses generated *)
+Definition genAddressesForCid (frecv_code : nat) (frecv_data : nat) cid :
+  G (list RiscMachine.address) :=
+  let how_many : nat := plus frecv_code frecv_data in
+  (* generate a 1ist of 10 addresses with generated block id and offset and given cid *)
+  liftGen
+    (List.map (fun '(bid,off) => SFI.address_of cid bid off))
+    (genBlockOffsetPairs frecv_code frecv_data).
+   
+
+(*******************************
+ * Env.E Generator
+ *******************************)
+
+Open Scope nat_scope.
+Definition genEForCid cid : G Env.E :=
+  liftGen (fun '(l1,l2) => List.combine l1 l2)
+          (liftGen2 pair
+                    (genAddressesForCid 10 0 cid)
+                    (* Procedure.id *)
+                    (liftGen (List.map Pos.of_nat) (vectorOf 10 (choose (0,100))))).
+Close Scope nat_scope.
+
+Definition foldE (ll : list Env.E) : Env.E :=
+  List.fold_left (fun l1 l2 => List.app l1 l2) ll nil.
+
+(* Q: How can I do the recursion on N, avoiding the strange 
+conversion to nat? *)
+Instance genE : Gen Env.E :=
+  {
+    arbitrary := 
+      let cids := List.map N.of_nat (List.seq 0 (N.to_nat SFI.COMP_MAX)) in
+      let generators := List.map genEForCid cids in
+      liftGen foldE (sequenceGen generators)
+  }.
+
+(*******************************
+ * Env Generator
+ *******************************)
+Instance genEnv : Gen Env.t :=
+  {
+    arbitrary := liftGen2 pair arbitrary arbitrary
+  }.
+
+Instance genReg : Gen RiscMachine.Register.t :=
+  {
+    arbitrary := elems [ RiscMachine.Register.R_ONE
+                         ; RiscMachine.Register.R_COM
+                         ; RiscMachine.Register.R_AUX1
+                         ; RiscMachine.Register.R_AUX2
+                         ; RiscMachine.Register.R_RA
+                         ; RiscMachine.Register.R_SP
+                         ; RiscMachine.Register.R_SFI_SP
+                         ; RiscMachine.Register.R_AND_CODE_MASK
+                         ; RiscMachine.Register.R_AND_DATA_MASK
+                         ; RiscMachine.Register.R_OR_CODE_MASK
+                         ; RiscMachine.Register.R_OR_DATA_MASK
+                         ; RiscMachine.Register.R_T
+                         ; RiscMachine.Register.R_D ]
+  }.
+
+
+(*******************************
+ * MachineState Generator
+ *******************************)
+Import RiscMachine.ISA.
+
+Instance genValue : Gen RiscMachine.value :=
+  {
+    arbitrary := arbitrary
+  }.
+
+Instance genImmediate : Gen RiscMachine.immediate :=
+  {
+    arbitrary := arbitrary
+  }.
+
+Instance genOp : Gen RiscMachine.ISA.binop :=
+  {
+    arbitrary := elems [ Addition
+                         ; Subtraction
+                         ; Multiplication
+                         ; Equality
+                         ; Leq
+                         ; BitwiseOr
+                         ; BitwiseAnd
+                         ; ShiftLeft
+                       ]
+  }.
+
+Definition genIConst : G instr :=
+  liftGen2 (fun (val : RiscMachine.value)
+                (reg : RiscMachine.Register.t) =>
+              IConst val reg ) arbitrary arbitrary.
+
+Definition gen2Reg (it :  RiscMachine.Register.t -> RiscMachine.Register.t -> instr) : G instr :=
+  liftGen2 (fun (r1 : RiscMachine.Register.t)
+                (r2 : RiscMachine.Register.t) =>
+              it r1 r2 ) arbitrary arbitrary.
+
+Definition genIBinOp : G instr :=
+  liftGen4 (fun (op : RiscMachine.ISA.binop)
+                (r1 : RiscMachine.Register.t)
+                (r2 : RiscMachine.Register.t)
+                (r3 : RiscMachine.Register.t) =>
+              IBinOp op r1 r2 r3) arbitrary arbitrary arbitrary arbitrary.
+
+Definition genIBnz : G instr :=
+  liftGen2 (fun (reg : RiscMachine.Register.t)
+                (imm : RiscMachine.immediate) =>
+              IBnz reg imm) arbitrary arbitrary.
+
+Definition genIJump : G instr :=
+  liftGen (fun (reg : RiscMachine.Register.t) => IJump reg) arbitrary.
+
+Definition genIJal (addresses : list RiscMachine.address) : G instr :=
+  elements INop (List.map
+                   (fun addr => IJal addr)
+                   addresses
+                ).
+
+Definition genInstr (addresses : list RiscMachine.address) : G instr :=
+  oneOf [ (returnGen INop)
+          ; genIConst
+          ; gen2Reg IMov
+          ; genIBinOp
+          ; gen2Reg ILoad
+          ; gen2Reg IStore
+          ; genIBnz
+          ; genIJump
+          ; genIJal addresses
+          ; (returnGen IHalt)
+        ].
+                         
+Definition genMemForAddresses (addresses : list RiscMachine.address) : G RiscMachine.Memory.t :=
+  let how_many : nat := List.length addresses in
+  liftGen (fun (lst : list (RiscMachine.address*(RiscMachine.value*RiscMachine.ISA.instr))) =>
+             List.fold_left
+                       (fun mem '(address, (val, i)) =>
+                          if ( SFI.is_code_address address)
+                          then RiscMachine.Memory.set_instr mem
+                                                            address
+                                                            i
+                          else RiscMachine.Memory.set_value mem
+                                                            address
+                                                            val)
+                       lst
+                       RiscMachine.Memory.empty
+                    )
+          (* list address*(val*instr) *)
+          ( liftGen (fun '(l1,l2) => List.combine addresses (List.combine l1 l2))
+                    (liftGen2 pair
+                              (vectorOf how_many arbitrary)
+                              (vectorOf how_many (genInstr addresses)))).
+  (* returnGen RiscMachine.Memory.empty. *)
+  
+
+Open Scope nat_scope.
+Instance genMem : Gen RiscMachine.Memory.t :=
+  {
+    arbitrary := 
+      let frecv_code := 50 in
+      let frecv_data := 50 in
+      let how_many : nat := frecv_code + frecv_data in
+      bindGen (genAddresses frecv_code frecv_data) genMemForAddresses
+  }.
+Close Scope nat_scope.
+                    
+(*
+Sample arbitrary.
+Check arbitrary.
+*)
